\documentclass[11pt,oneside,a4paper]{article}
\author{黄国鹏}
\usepackage{ctex}
\usepackage{graphicx}
\usepackage{tabularray}
\usepackage{tagging}
\usepackage{amsthm}
\usepackage{amsmath}
\title{软件理论基础第三次作业 }
\begin{document}
\maketitle
\begin{enumerate}
    \item 利用$L$的完备性定理证明以下各式成立
    \begin{enumerate}
        \item[(1)] $\vdash \neg(A \rightarrow B) \rightarrow(B \rightarrow A)$
        证：由逻辑等价：
        \[\begin{array}{l}
            \neg (A \to B) \to (B \to A)\\
             = \neg \neg (A \to B) \vee (B \to A)\\
             = (\neg A \vee B) \vee (\neg B \vee A)\\
             = \neg A \vee A \vee B \vee \neg B\\
             = 1
            \end{array}\]
        任取$v \in \Omega$,有$v(\neg (A \to B) \to (B \to A))=1$
        
        因此$\models \neg (A \to B) \to (B \to A)$

        由完备性定理$\vdash \neg(A \rightarrow B) \rightarrow(B \rightarrow A)$


        \item[(2)]$((A \vee B) \rightarrow C) \approx(A \rightarrow C) \wedge(B \rightarrow C)$
        
        证：由逻辑等价：
        \[\begin{array}{l}
              (A \vee B) \to C\\
             = \neg (A \vee B) \vee C\\
             = (\neg A \wedge \neg B) \vee C\\
             = (\neg A \vee C) \wedge (\neg B \vee C)\\
             = (A \to C) \wedge (B \to C)
            \end{array}\]
        任取$v \in \Omega$,有$v((A \vee B) \to C) = v((A \to C) \wedge (B \to C))$

        因此$\models ((A \vee B) \rightarrow C) \to (A \rightarrow C) \wedge(B \rightarrow C)$

        由完备性定理$\vdash ((A \vee B) \rightarrow C) \to (A \rightarrow C) \wedge(B \rightarrow C)$

        同理可得$ \vdash ((A \to C) \wedge (B \to C)) \to ((A \vee B) \to C)$

        因此可得$((A \vee B) \rightarrow C) \approx(A \rightarrow C) \wedge(B \rightarrow C)$
        证毕


        \item[(3)]$((A \wedge B) \rightarrow C) \approx(A \rightarrow C) \vee(B \rightarrow C)$
        
        证：由逻辑等价：
        \[\begin{array}{l}
            (A \wedge B) \to C\\
             = (\neg (A \wedge B) \vee C)\\
             = \neg A \vee \neg B \vee C\\
             = \neg A \vee \neg B \vee C \vee C\\
             = \neg A \vee C \vee \neg B \vee C\\
             = (A \to C) \vee (B \to C)
            \end{array}\]
        任取$v \in \Omega$,有$v((A \wedge B) \to C) = v((A \to C) \vee (B \to C))$

        因此$\models ((A \wedge B) \to C) \to ((A \to C) \vee (B \to C))$

        由完备性定理$\vdash ((A \wedge B) \to C) \to ((A \to C) \vee (B \to C))$
        
        同理可得$ \vdash ((A \to C) \vee (B \to C)) \to ((A \wedge B) \to C)$

        因此可得$((A \wedge B) \rightarrow C) \approx(A \rightarrow C) \vee(B \rightarrow C)$
        证毕






    \end{enumerate}
    \item 
\end{enumerate}
\end{document}